\documentclass{ximera}
\input{../../preamble.tex}

\begin{document}

In Exercises \ref{YZ_1.3_decomp2}-\ref{YZ_1.3_decomp3}, use \eqref{YZ_2.1_decomp} to express $A=B+C$, where $B$ is symmetric and $C$ is skew-symmetric.

\begin{exercise}\label{YZ_1.3_decomp2}
$A=\Matrix{1&9\\3&2}$.

\begin{solution}
\ans $A=\Matrix{1&6\\6&2}+\Matrix{0&3\\-3&0}$.

\soln We compute $\frac{A+A^t}{2}$, which is equal to 
\[
\frac12\Matrix{1&9\\3&2}+\frac12\Matrix{1&3\\9&2}=\Matrix{1&6\\6&2}.
\]
We compute $\frac{A-A^t}{2}$, which is equal to 
\[
\frac12\Matrix{1&9\\3&2}-\frac12\Matrix{1&3\\9&2}=\Matrix{0&3\\-3&0}.
\]
So we express $A=\Matrix{1&6\\6&2}+\Matrix{0&3\\-3&0}$ as a sum of a symmetric matrix and a skew-symmetric matrix.
\end{solution}
\end{exercise}


\begin{exercise}\label{YZ_1.3_decomp3}
$A=\Matrix{0&3&-4\\3&9&-1\\1&6&-4}$. 

\begin{solution}
\ans $A=\Matrix{0&3&-3/2\\3&9&5/2\\-3/2&5/2&-4}+\Matrix{0&0&-5/2\\0&0&-7/2\\5/2&7/2&0}$.

\soln
We compute $\frac{A+A^t}{2}$, which is equal to 
\[
\frac{1}{2}\Matrix{0&3&-4\\3&9&-1\\1&6&-4}+\frac{1}{2}\Matrix{0&3&1\\3&9&6\\-4&-1&-4}=\Matrix{0&3&-3/2\\3&9&5/2\\-3/2&5/2&-4}.
\]
We compute $\frac{A-A^t}{2}$, which is equal to 
\[
\frac{1}{2}\Matrix{0&3&-4\\3&9&-1\\1&6&-4}-\frac{1}{2}\Matrix{0&3&1\\3&9&6\\-4&-1&-4}=\Matrix{0&0&-5/2\\0&0&-7/2\\5/2&7/2&0}.
\]
So can express $A=\Matrix{0&3&-3/2\\3&9&5/2\\-3/2&5/2&-4}+\Matrix{0&0&-5/2\\0&0&-7/2\\5/2&7/2&0}$
as a sum of a symmetric matrix and a skew-symmetric matrix.

\end{solution}
\end{exercise}

\end{document}