\documentclass{ximera}
\input{../../preamble.tex}
\begin{document}




\begin{exercise} \label{YZ_3.4.7}
Let $L:\mathbb R^3\to \mathbb R^2$ be a linear mapping such that 
\[
L\Matrix{1\\-1\\0}=\Matrix{-3\\1},~L\Matrix{0\\1\\1 }=\Matrix{2\\-1},
\]
and 
\[
L\Matrix{ 0\\1\\-1}=\Matrix{0\\1}.
\]


\begin{enumeratea}
\item Determine the matrix representation of $L$. Namely, find the matrix $A$ such that $L_A=L$.

\item Verify that  $\Matrix{0\\2\\-2}$ is a solution to $Lx=\Matrix{0\\2}$
\item Find the full set of solutions of $Lx=\Matrix{0\\2}$.
\end{enumeratea}


\begin{solution}

\ans 
\begin{enumeratea}
\item  The matrix representation of $L$ is 
 \[
\Matrix{ -2&1&1\\1&0&-1}.
\]

\item Direct verification.
\item The general solution of the inhomogeneous equation is 
\[
\alpha \Matrix{1\\1\\1}+\Matrix{0\\2\\-2}, \alpha\in \mathbb R
\]

\end{enumeratea}



\soln 

\begin{enumeratea}
\item  $\Matrix{ 0\\0\\2 }=L\Matrix{ 0\\1\\1}-L\Matrix{0\\1\\-1}=\Matrix{2\\-2 }$, so 
\[
L\Matrix{0\\0\\1}=\Matrix{1\\-1}.
\]
Similarly, subtracting it from the second equation, we get 
\[
L\Matrix{0\\1\\0}=L\Matrix{ 0\\1\\1}-L\Matrix{0\\0\\1}=\Matrix{2\\-1}-\Matrix{1\\-1}=\Matrix{1\\0 }.
\]

Finally, adding it to the first equation, we have 
\[
L\Matrix{1\\0\\0}=L\Matrix{1\\-1\\0}+L\Matrix{0\\1\\0}=\Matrix{ -3\\1}+\Matrix{1\\0}=\Matrix{-2\\1}.
\]

Therefore the matrix representation $A$ of $L$ is 
\[
\Matrix{ -2&1&1\\1&0&-1}.
\]

\item Verify that 
\[
\Matrix{ -2&1&1\\1&0&-1} \Matrix{0\\2\\-2} =\Matrix{0\\2}.
\]


\item From the elementary row reduction of $A$, one can find the solution to $Ax=0$ is 
\[
\Matrix{1\\1\\1}.
\]
Therefore, the general solution of the inhomogeneous equation is 
\[
\alpha \Matrix{1\\1\\1}+\Matrix{0\\2\\-2}, \alpha\in \mathbb R
\]
\end{enumeratea}



\end{solution}
\end{exercise}








\end{document}
