\documentclass{ximera}
\input{../../preamble.tex}
\begin{document}
\begin{exercise} \label{c4.7.3}
Let
\[
A=\mattwo{1}{2}{-1}{-1} \AND B =\mattwo{2}{3}{1}{4}.
\]
Compute $AB$ and $B^tA^t$.  Verify that $(AB)^t=B^tA^t$ for these
matrices $A$ and $B$.

\begin{solution}
\soln 
First compute $AB$:
\[ 
\mattwo{1}{2}{-1}{-1}\mattwo{2}{3}{1}{4} = \mattwo{4}{11}{-3}{-7} 
\]
then take its transpose.
\[ 
(AB)^t = \mattwo{4}{-3}{11}{-7}. 
\]
Then calculate
\[ 
B^tA^t = \mattwo{1}{-1}{2}{-1}\mattwo{2}{1}{3}{4} = \mattwo{4}{-3}{11}{-7}. 
\]
So $(AB)^t = B^tA^t$ for these matrices $A$ and $B$.
\end{solution}
\end{exercise}
\end{document}
