\documentclass{ximera}
\input{../../preamble.tex}


\begin{document}


Let $a=1+i$ and $b=\sqrt{3}-i$. In Exercise \ref{YZ_2.5_CplxBasic1}-\ref{YZ_2.5_CplxBasic4}, simplify the given expression.
\begin{exercise} \label{YZ_2.5_CplxBasic1}
$a+b$.

\begin{solution}
\ans $1+\sqrt{3}$.

\soln $a+b=1+i+\sqrt{3}-i=(1+\sqrt{3})+i(1-1)=1+\sqrt{3}$.

\end{solution}
\end{exercise}

\begin{exercise}\label{YZ_2.5_CplxBasic2}
$b-3a$.

\begin{solution}
\ans $(\sqrt{3}-3)-4i$.

\soln $b-3a=\sqrt{3}-i-3(1+i)=(\sqrt{3}-3)+i(-1-3)=(\sqrt{3}-3) - 4i$.
\end{solution}
\end{exercise}

\begin{exercise}\label{YZ_2.5_CplxBasic3}
$\frac{1}{a}$.

\begin{solution}
\ans $\frac{1-i}{2}$.

\soln $\frac1a=\frac{1}{1+i}=\frac{1-i}{(1+i)(1-i)}=\frac{1-i}{2}$.
\end{solution}
\end{exercise}


\begin{exercise}\label{YZ_2.5_CplxBasic4}
$a\bar{b}$.

\begin{solution}
\ans $(\sqrt{3}-1)+i(\sqrt{3}+1)$.

\soln $a\bar{b}=(1+i)(\sqrt{3}+i)=(\sqrt{3}-1) + i(\sqrt{3}+1)$.
\end{solution}
\end{exercise}





\end{document}



